Make compatible with latest Coq trunk (needed because of new type class fixes). In interfaces/universal_algebra: remove unused things, clean up, better names, more documentation.

interfaces/universal_algebra.v
@@ -4,211 +4,140 @@ Require Import
   Morphisms Setoid Program List
   abstract_algebra theory.categories util.
 
-Section with_atomic. Variable Atomic: Set.
+Record Entailment (P: Type): Type := { entailment_premises: list P; entailment_conclusion: P }.
+
+Section with_sorts. Variable Sorts: Set.
+
+  (* For single-sorted algebras, Sorts will typically be unit. *)
+
+  (* OpType describes the type of an operation in an algebra. Note that higher order function types are excluded: *)
 
   Inductive OpType: Set :=
-    | constant (a: Atomic)
-    | function (a: Atomic) (g: OpType).
+    | constant (a: Sorts)
+    | function (a: Sorts) (g: OpType).
 
-  Definition op_type (T: Atomic -> Type): OpType -> Type :=
-    fix F (t: OpType): Type :=
-      match t with
-      | constant a => T a
-      | function a g => T a -> F g
+  Section with_sort_realizations. Variable Sort: Sorts -> Type.
+
+    (* Given a Type for each sort, we can map the operation type descriptions to real function types: *)
+
+    Fixpoint op_type (o: OpType): Type :=
+      match o with
+      | constant a => Sort a
+      | function a g => Sort a -> op_type g
       end.
 
-  Definition prop (T : Atomic -> Type) (P : forall a : Atomic, T a -> Prop) :=
-    fix F (o0 : OpType) : op_type T o0 -> Prop :=
-      match o0 with
-      | constant a => P a
-      | function a g => fun X => forall x, F g (X x)
-      end.
+    (* We use extensional equivalence for such generated function types: *)
 
-  Definition gen_op_type (Arg Res: Atomic -> Type): OpType -> Type :=
-    fix F (t: OpType): Type :=
-      match t with
-      | constant a => Res a
-      | function a g => Arg a -> F g
-      end. (* used in initiality proof for w *)
+    Context `{e: forall s, Equiv (Sort s)}.
 
-  Section with_atomic_inter. Variable T: Atomic -> Type.
-
-    Definition op_type_equiv
-       `{e: forall A, Equiv (T A)}: forall o: OpType, Equiv (op_type T o) :=
-     fix F (o: OpType): Equiv (op_type T o) :=
-      match o return Equiv (op_type T o) with
+    Fixpoint op_type_equiv o: Equiv (op_type o) :=
+      match o with
       | constant A => e A
-      | function A g => (e A ==> F g)%signature
+      | function A g => (e A ==> op_type_equiv g)%signature
       end.
 
-    Definition gen_op_type_equiv (T': Atomic -> Type)
-       `{e: forall A, Equiv (T A)}
-       (he: forall A, T A -> T' A -> Prop) :=
-     fix F (o: OpType): op_type T o -> gen_op_type T T' o -> Prop :=
-      match o return op_type T o -> gen_op_type T T' o -> Prop with
-      | constant A => he A
-      | function A g => fun x y => forall i j, i == j -> F g (x i) (y j) (*(e A ==> F g)%signature*)
-      end.
+    Global Existing Instance op_type_equiv. (* There's no [Global Instance Fixpoint]. *)
 
-    Definition gen_op_type_equiv' (T': Atomic -> Type)
-       `{e: forall A, Equiv (T A)}
-       (he: forall A, T A -> T' A -> Prop) :=
-     fix F (o: OpType): op_type T o -> gen_op_type T' T o -> Prop :=
-      match o return op_type T o -> gen_op_type T' T o -> Prop with
-      | constant A => e A
-      | function A g => fun x y => forall i j, he _ i j -> F g (x i) (y j) (*(e A ==> F g)%signature*)
-      end.
+    Global Instance sig_type_sym `{forall s, Symmetric (e s)}: Symmetric (op_type_equiv o).
+    Proof. induction o; simpl; firstorder. Qed.
+    
+    (* We need either reflexivity or symmetry of e in order to get transitivity of op_type_equiv: *)
 
-    Global Existing Instance op_type_equiv.
-
-    (* op_type_equiv is /almost/ an equivalence relation. Note that it is /not/ readily reflexive. *)
-
-    Global Instance sig_type_trans `{e: forall A, Equiv (T A)}
-      `{forall A, Reflexive (e A)} `{forall A, Transitive (e A)}: Transitive (op_type_equiv o).
+    Global Instance sig_type_trans `{forall s, Reflexive (e s)} `{forall s, Transitive (e s)}: Transitive (op_type_equiv o).
     Proof. induction o; simpl; firstorder. Qed.
 
-      (* curiously, having symmetry is also sufficient enough to get transitivity: *)
-    Global Instance sig_type_trans' `{e: forall A, Equiv (T A)}
-       `{forall A, Symmetric (e A)}
-       `{forall A, Transitive (e A)}: Transitive (op_type_equiv o).
-    Proof.
-     induction o.
-     apply H0.
-     repeat intro.
-     transitivity (y y0). apply (H1 x0 _ H3).
+    Global Instance sig_type_trans' `{forall s, Symmetric (e s)} `{forall s, Transitive (e s)}: Transitive (op_type_equiv o).
+    Proof with auto.
+     induction o; simpl...
+     intros x y ? ? H2 x0 y0 ?.
+     transitivity (y y0)...
      apply H2.
-     transitivity x0; [symmetry |]; assumption.
+     transitivity x0; [symmetry |]...
     Qed.
 
-    Global Instance sig_type_sym `{e: forall A, Equiv (T A)} `{forall A, Symmetric (e A)}: Symmetric (op_type_equiv o).
-    Proof. induction o; simpl; firstorder. Qed.
-
-    Lemma sig_type_refl `{e: forall A, Equiv (T A)} `{forall a, Reflexive (e a)} (o: OpType) a (x: op_type T (function a o)) y:
+      (* This is the closest i've been able to get to reflexivity thus far: *)
+    Lemma sig_type_refl `{forall a, Reflexive (e a)} (o: OpType) a (x: op_type (function a o)) y:
       Proper equiv x ->
       op_type_equiv o (x y) (x y).
-    Proof.
-     intros.
-     apply (H0 y y).
-     reflexivity.
-    Qed.
+    Proof. intro H0. apply H0. reflexivity. Qed.
 
-  End with_atomic_inter.
+  End with_sort_realizations.
 
   Section map_op.
 
-    (* Given maps between two sets of atomics, there are maps between the corresponding op_types*)
+    (* Given maps between two realizations of the sorts, there are maps between the corresponding op_types*)
 
-    Context {A B: Atomic -> Type} `{forall a, Equiv (A a)} `{forall a, Equiv (B a)}
-     (ab: forall a, A a -> B a) (ba: forall a, B a -> A a)
-     `{forall a, Proper (equiv ==> equiv) (ab a)}
-     `{forall a, Proper (equiv ==> equiv) (ba a)}.
+    Context {A B: Sorts -> Type}
+      `{forall a, Equiv (A a)} `{forall a, Equiv (B a)}
+      (ab: forall a, A a -> B a)
+      (ba: forall a, B a -> A a)
+      `{forall a, Proper (equiv ==> equiv) (ab a)}
+      `{forall a, Proper (equiv ==> equiv) (ba a)}.
 
     Fixpoint map_op {o: OpType}: op_type A o -> op_type B o :=
       match o return op_type A o -> op_type B o with
       | constant u => ab u
-      | function u v => fun x => fun y => map_op (x (ba u y))
+      | function _ _ => fun x y => map_op (x (ba _ y))
       end.
 
     Global Instance map_op_proper o: Proper (op_type_equiv A o ==> op_type_equiv B o) (@map_op o).
     Proof. induction o; simpl; firstorder. Qed.
+      (* todo: can't we make this nameless? *)
 
   End map_op.
 
-  Context {A B: Atomic -> Type} {e: forall a, Equiv (B a)} `{forall b, Equivalence (e b)} 
+  (* If the maps between the sorts are eachother's inverse, then so are the two generated op_type maps: *)
+
+  Context {A B: Sorts -> Type} {e: forall a, Equiv (B a)} `{forall b, Equivalence (e b)} 
    (ab: forall a, A a -> B a) (ba: forall a, B a -> A a) 
    `(iso: forall a (x: B a), ab a (ba a x) == x).
 
   Lemma map_iso o (x: op_type B o) (xproper: Proper equiv x): map_op ab ba (map_op ba ab x) == x.
   Proof with auto; try reflexivity.
    induction o; simpl; intros...
-   repeat intro.
+   intros x0 y H0.
    change (map_op ab ba (map_op ba ab (x (ab a (ba a x0)))) == x y).
    transitivity (x (ab a (ba a x0))).
     apply IHo, xproper...
    apply xproper. rewrite iso, H0...
   Qed.
 
-End with_atomic.
+End with_sorts.
 
 Inductive Signature: Type :=
-  { sign_op:> Set
-  ; sign_atomics: Set
-  ; sign_sig:> sign_op -> OpType sign_atomics }.
+  { sorts: Set
+  ; operation:> Set
+  ; operation_type:> operation -> OpType sorts }.
+
+(* We now introduce additional things in order to let us eventually define equational theories and varieties. *)
 
 Section for_signature. Variable sign: Signature.
 
-  Class Implementation (A: sign_atomics sign -> Type) := op: forall o, op_type _ A (sign o).
+  Let sorts := sorts sign.
+  Let OpType := OpType sorts.
 
-  Class Propers (A: sign_atomics sign -> Type) `{forall a, Equiv (A a)} `{Implementation A} :=
-    propers:> forall o: sign, Proper (op_type_equiv _ A (sign o)) (op o).
+  (* An implementation of a signature for a given realization of the sorts is simply a function (of the right type) for each operation: *)
 
-  Inductive Term (V: Set): OpType (sign_atomics sign) -> Set :=
-    | Var (v: V) (a: sign_atomics sign): Term V (constant _ a)
-    | App (t: OpType (sign_atomics sign)) y: Term V (function _ y t) -> Term V (constant _ y) -> Term V t
-    | Op (o: sign): Term V (sign o).
+  Class Implementation (A: sorts -> Type) := op: forall o, op_type _ A (sign o).
 
-  Implicit Arguments Var [[V]].
+  (* And we'll usually want to work with proper implementations: *)
 
-  Let T := Term nat.
-  Definition Identity t := prod (T t) (T t).
-  Definition Term0 sort := T (constant _ sort).
-  Definition Identity0 sort := Identity (constant _ sort).
-    (* While Identity0 is the one we usually have in mind, the generalized version for arbitrary op_types
-     is required to make induction proofs work. The same is (more or less) true for Term/Term0. *)
+  Class Propers (A: sorts -> Type) `{forall a, Equiv (A a)} `{Implementation A} :=
+    propers:> forall o: sign, Proper equiv (op o). (* This equiv is op_type_equiv defined above. *)
 
-  Definition mkIdentity0 {sort}: T (constant _ sort) -> T (constant _ sort) -> Identity0 sort := pair.
-
-  Inductive Statement: Type :=
-    | Eq t (i: Identity t)
-    | Impl (a b: Statement)
-    | Conj (a b: Statement)
-    | Ext (P: Prop).
-
-  (* Note: The statements above are too liberal (i.e. not equational) to support product varieties. *)
-
-  Record Entailment (P: Type): Type := { entailment_premises: list P; entailment_conclusion: P }.
-
-  Definition EqEntailment := Entailment (sigT Identity0).
-
-  Definition identity_as_eq (s: sigT Identity0): Statement := Eq _ (projT2 s).
-  Coercion identity_as_entailment sort (e: Identity0 sort): EqEntailment := Build_Entailment _ nil (existT _ _ e).
-
-  Coercion entailment_as_statement (e: EqEntailment): Statement :=
-     (fold_right Impl (identity_as_eq (entailment_conclusion _ e)) (map identity_as_eq (entailment_premises _ e))).
-
-  Definition boring_entailment_as_statement (e: EqEntailment): Statement :=
-    Impl (fold_right Conj (Ext True) (map identity_as_eq (entailment_premises _ e))) 
-      (identity_as_eq (entailment_conclusion _ e)).
-
-
-  Fixpoint propje V (P: forall a, Term V (constant _ a) -> Prop) {ot}: Term V ot -> Prop :=
-    match ot with
-    | constant x => P x
-    | function x y => fun z => forall v, P _ v -> propje V P (App V _ _ z v)
-    end.
-
-  Lemma indu V (P: forall a, Term V (constant _ a) -> Prop):
-    (forall o a (t: Term V (constant _ a)) (t0: Term V (function (sign_atomics sign) a o)),
-       P _ t -> propje V P t0 -> propje V P (App _ _ _ t0 t)) ->
-    (forall v a, P _ (Var v a)) ->
-    (forall o, propje V P (Op _ o)) ->
-    forall a (t: Term V (constant _ a)), P a t.
-  Proof.
-   intros.
-   cut (propje V P t). intuition.
-   induction t; simpl; intuition.
-  Qed.
-    (* Todo: Rename and explain propje/indu. *)
+  (* As an aside: given two implementations in different realizations of the sorts, and a map between
+   them for each sort, we can say what it means for that map to preserve the algebra's operations,
+   i.e. what it takes for it to be a homomorphism: *)
 
   Section for_map.
 
-    Context (A: sign_atomics sign -> Type) (B: sign_atomics sign -> Type)
+    Context (A B: sorts -> Type)
       `{ea: forall a, Equiv (A a)} `{eb: forall a, Equiv (B a)}
       `{!Implementation A} `{!Implementation B} (f: forall a, A a -> B a).
 
     Implicit Arguments f [[a]].
 
-    Fixpoint Preservation {n: OpType (sign_atomics sign)}: op_type _ A n -> op_type _ B n -> Prop :=
+    Fixpoint Preservation {n: OpType}: op_type _ A n -> op_type _ B n -> Prop :=
       match n with
       | constant d => fun o o' => f o == o'
       | function x y => fun o o' => forall x, Preservation (o x) (o' (f x))
@@ -229,14 +158,104 @@ Section for_signature. Variable sign: Signature.
 
   End for_map.
 
+  (* Proceeding on our way toward equational theories and varieties, we define terms: *)
+
+  Inductive Term (V: Set): OpType -> Set :=
+    | Var (v: V) (a: sorts): Term V (constant _ a)
+    | App (t: OpType) y: Term V (function _ y t) -> Term V (constant _ y) -> Term V t
+    | Op (o: sign): Term V (sign o).
+
+  Implicit Arguments Var [[V]].
+
+  (* Term has OpType as an index, which means we can have terms with function
+   types (no surprise there). However, often we want to prove properties that only speak of
+   terms of arity 0 (that is, terms of type [Term (constant _ sort)] for some sort): *)
+
+  Definition Term0 v sort := Term v (constant _ sort).
+
+  Section applications_ind.
+
+    Context (V: Set) (P: forall a, Term0 V a -> Prop).
+
+    (* To be able to prove such a P by induction, we must first transform it into a statement
+     about terms of all arities. Roughly speaking, we do this by saying
+     [forall x0...xN, P (App (... (App f x0) ...) xN)] for a term f of arity N. *)
+
+    Fixpoint applications {ot}: Term V ot -> Prop :=
+      match ot with
+      | constant x => P x
+      | function x y => fun z => forall v, P _ v -> applications (App V _ _ z v)
+      end.
+
+    (* To prove P/applications by induction, we can then use: *)
+
+    Lemma applications_ind:
+      (forall o a t t', P a t -> applications t' -> applications (App _ o a t' t)) ->
+      (forall v a, P _ (Var v a)) ->
+      (forall o, applications (Op _ o)) ->
+      forall a t, P a t.
+    Proof with intuition. intros. cut (applications t)... induction t; simpl... Qed.
+
+  End applications_ind.
+
+  (* We parameterized Term over the index set for variables, because we will
+   wants terms /with/ variables when speaking of identities in equational theories,
+   but will want terms /without/ variables when constructing initial objects
+   in variety categories generically in theory/ua_initial (which we get by taking
+   False as the variable index set). *)
+   
+  Definition T := Term nat.
+  Definition T0 := Term0 nat.
+
+  Definition Identity t := prod (T t) (T t).
+  Definition Identity0 sort := Identity (constant _ sort).
+    (* While Identity0 is the one we usually have in mind, the generalized version for arbitrary op_types
+     is required to make induction proofs work. *)
+
+  Definition mkIdentity0 {sort}: T (constant _ sort) -> T (constant _ sort) -> Identity0 sort := pair.
+
+  (* The laws in an equational theory will be entailments of identities for any of the sorts: *)
+
+  Definition EqEntailment := Entailment (sigT Identity0).
+
+  (* We also introduce a more general class of statements that we use to conveniently transfer
+   statements between different models of a variety: *)
+
+  Inductive Statement: Type :=
+    | Eq t (i: Identity t)
+    | Impl (a b: Statement)
+    | Conj (a b: Statement)
+    | Ext (P: Prop).
+
+  (* Statements are a strict generalization of EqEntailments. We cannot use the former for the laws,
+   though, because they are too liberal (i.e. not equational) to support product varieties.
+   We do have two injections: *)
+
+  Definition identity_as_eq (s: sigT Identity0): Statement := Eq _ (projT2 s).
+  Coercion identity_as_entailment sort (e: Identity0 sort): EqEntailment := Build_Entailment _ nil (existT _ _ e).
+
+  Coercion entailment_as_statement (e: EqEntailment): Statement :=
+     (fold_right Impl (identity_as_eq (entailment_conclusion _ e)) (map identity_as_eq (entailment_premises _ e))).
+
+  Definition entailment_as_conjunctive_statement (e: EqEntailment): Statement :=
+    Impl (fold_right Conj (Ext True) (map identity_as_eq (entailment_premises _ e))) 
+      (identity_as_eq (entailment_conclusion _ e)).
+
+  (* The first one (the coercion) converts an entailment of the form (A, B, C |- D) into a statement of
+   the form (A -> B -> C -> D), while the second converts the same entailment into a statement of
+   the form ((A /\ B /\ C) -> D). Both have their uses in induction proofs. *)
+
+  (* To be able to state that laws hold in a model of a variety, we must be able to evaluate terms
+   using the model's implementation and using arbitrary variable assignments: *)
+
   Section Vars.
 
-    Context (A: sign_atomics sign -> Type) (V: Set) `{e: forall a, Equiv (A a)} `{forall a, Equivalence (e a)}.
+    Context (A: sorts -> Type) (V: Set) `{e: forall a, Equiv (A a)} `{forall a, Equivalence (e a)}.
 
     Definition Vars := forall a, V -> A a.
 
     Global Instance: Equiv Vars :=
-     @pointwise_dependent_relation (sign_atomics sign) (fun a => V -> A a)
+     @pointwise_dependent_relation sorts (fun a => V -> A a)
       (fun _ => pointwise_relation _ equiv).
 
     Global Instance: Equivalence (equiv: relation Vars).
@@ -248,17 +267,14 @@ Section for_signature. Variable sign: Signature.
     Context
      `{ea: forall a, Equiv (A a)} `{!forall a, Equivalence (ea a)} `{!Implementation A} `{@Propers A ea _}.
 
-    Fixpoint eval {V} {n: OpType (sign_atomics sign)} (vars: Vars A V) (t: Term V n) {struct t}:
-        op_type _ A n :=
+    Fixpoint eval {V} {n: OpType} (vars: Vars A V) (t: Term V n) {struct t}: op_type _ A n :=
       match t in Term _ n return op_type _ A n with
       | Var v a => vars a v
       | Op o => op o
       | App n a f p => eval vars f (eval vars p)
       end.
  
-    Let bla := op_type_equiv (sign_atomics sign) A.
-
-    Global Instance eval_proper {V} (n: OpType (sign_atomics sign)):
+    Global Instance eval_proper {V} (n: OpType):
       Proper (equiv ==> eq ==> equiv) (@eval V n).
     Proof with auto.
      intros x y E a _ [].
@@ -270,46 +286,43 @@ Section for_signature. Variable sign: Signature.
 
     Definition eval_stmt (vars: Vars A nat): Statement -> Prop :=
       fix F (s: Statement) :=
-      match s with
-      | Eq _ i => eval vars (fst i) == eval vars (snd i)
-      | Impl a b => F a -> F b
-      | Ext P => P
-      | Conj a b => F a /\ F b
-      end.
+       match s with
+       | Eq _ i => eval vars (fst i) == eval vars (snd i)
+       | Impl a b => F a -> F b
+       | Ext P => P
+       | Conj a b => F a /\ F b
+       end.
 
     Global Instance eval_stmt_proper: Proper (equiv ==> eq ==> iff) eval_stmt.
     Proof with auto.
      intros v v' ve s s' se. subst.
      induction s'; simpl; intuition.
       transitivity (eval v (fst i)).
-       rewrite <- ve.
-       unfold equiv.
-       unfold bla.
-       apply eval_proper...
-       reflexivity.
+       apply eval_proper... symmetry...
       transitivity (eval v (snd i))...
       apply eval_proper...
      transitivity (eval v' (fst i)).
       apply eval_proper...
      rewrite H1.
-     apply eval_proper...
-     symmetry...
-    Qed. (* todo: clean up *)
+     apply eval_proper... symmetry...
+    Qed.
 
     Definition boring_eval_entailment (vars: Vars A nat) (e: EqEntailment):
-      eval_stmt vars e <-> eval_stmt vars (boring_entailment_as_statement e).
+      eval_stmt vars e <-> eval_stmt vars (entailment_as_conjunctive_statement e).
     Proof. destruct e. simpl. induction entailment_premises0; simpl; intuition. Qed.
 
   End eval.
 
 End for_signature.
 
+(* And with that, we define equational theories and varieties: *)
+
 Record EquationalTheory :=
   { et_sig:> Signature
   ; et_laws:> EqEntailment et_sig -> Prop }.
 
 Record Variety (et: EquationalTheory): Type := MkVariety
-  { variety_atomics:> sign_atomics et -> Type
+  { variety_atomics:> sorts et -> Type
   ; variety_equiv: forall a, Equiv (variety_atomics a)
   ; variety_op:> Implementation et variety_atomics
   ; variety_equivalence: forall a, Equivalence (variety_equiv a)
